denotational/Ltac.v
@@ -1,0 +1,36 @@
+From CTree Require Import CTree SBisim Equ.
+
+Ltac fold_bind :=
+  lazymatch goal with
+  | [ |- sbisim _ (CTree.subst ?k ?t) ] => fold (CTree.bind t k)
+  | [ H: context[CTree.subst ?f ?x] |- _ ] => fold (CTree.bind x f) in H
+  | [ |- context[CTree.subst ?f ?x] ] => fold (CTree.bind x f) in *
+  end.
+
+(** Main lemma, C1 is bisimilar to C2 *)
+Ltac sb_fwd_I := setoid_rewrite ctree_eta;
+                 repeat (cbn; multimatch goal with
+                              | [ |- sbisim (CTree.bind ?t _) (CTree.bind ?t _) ] =>
+                                  apply sbisim_clo_bind
+                                        
+                              | [ |- sbisim (Ret _) (Ret _) ] => apply sb_ret
+                              | [ |- context[sbisim (TauI _) _] ] => rewrite !sb_tauI
+
+                              | [ |- context[CTree.bind (Ret _) _] ] => rewrite ?bind_ret_l
+                              | [ |- context[CTree.bind (CTree.bind _ _) _]] => rewrite ?bind_bind
+                              | [ x: fin _ |- _] => dependent destruction x; subst
+                              | [ |- context[ChoiceI 1 _]] => rewrite sb_choiceI1
+                              | [ |- sbisim (ChoiceI ?n _) ?R ] =>
+                                  lazymatch R with
+                                  | ChoiceI ?n _ => apply sb_choiceI_id; intros
+                                  | ChoiceV _ _ => fail "Canot unify visible and invisilble states"
+                                  | _ => rewrite sb_choiceI_idempotent; intros
+                                  end
+                              (** Symmetric patterns *)
+                              | [ |- sbisim ?L (ChoiceI ?n _) ] =>
+                                  lazymatch L with
+                                  | ChoiceI ?n _ => apply sb_choiceI_id; intros
+                                  | ChoiceV _ _ => fail "Canot unify visible and invisilble states"
+                                  | _ => rewrite sb_choiceI_idempotent; intros
+                                  end
+                              end; idtac "."; repeat fold_bind).
